pushing changes before refactor to final proof (constraining program field when running instD as part of elle sem

elle/ElleCorrect/ElleAltSemantics.thy
@@ -141,6 +141,7 @@ wrap in a Seq [] *)
     cp_next t cp = Some cp' \<Longrightarrow>
     elle_alt_sem t i cp' z z' \<Longrightarrow>
     elle_alt_sem t i cp z z'"
+(* end vs not end *)
 (* nonempty sequence *)
 | "\<And> t cp x e h rest z z' .
     ll_get_node t cp = Some (x, LSeq e (h#rest)) \<Longrightarrow>
@@ -203,6 +204,8 @@ fun ll4_load_cctx :: "constant_ctx \<Rightarrow> ll4 \<Rightarrow> constant_ctx"
       \<rparr>)"
 
 (* based on ProgramList.program_list_of_lst *)
+(* idea: here, we validate the STACK sizes *)
+(* TODO: separate out the validation phase *)
 fun  program_list_of_lst_validate  :: "inst list \<Rightarrow> inst list option"  where 
  " program_list_of_lst_validate [] = Some []"
 |" program_list_of_lst_validate (Stack (PUSH_N bytes) # rest) =
@@ -229,6 +232,8 @@ fun ll4_load_lst_cctx :: "constant_ctx \<Rightarrow> ll4 \<Rightarrow> constant_
       Evm.program.make (\<lambda> i . index (program_list_of_lst (codegen' t)) (nat i))
                        (length (program_list_of_lst (codegen' t)))\<rparr>)"
 
+(* codegen check checks to make sure stack instructions match their length *)
+(* load_lst_validate makes sure there are no pushes <1 or >32 bytes *)
 fun ll4_load_lst_validate :: "constant_ctx \<Rightarrow> ll4 \<Rightarrow> constant_ctx option" where
 "ll4_load_lst_validate cc t =
   (case codegen'_check t of None \<Rightarrow> None
@@ -498,6 +503,26 @@ next
 done
 qed
 
+lemma qvalid_desc_bounded1 [rule_format] :
+"((a, (t :: ('a, 'b, 'c, 'd, 'e, 'f, 'g) llt)) \<in> ll_valid_q \<longrightarrow>
+ (! cp nd nd' desc . ll_get_node (a, t) cp = Some ((nd, nd'), desc) \<longrightarrow>
+    nd \<ge> fst a \<and> nd' \<le> snd a))"
+  apply(insert qvalid_desc_bounded')
+  apply(fastforce)
+  done
+
+lemma qvalid_desc_bounded2 [rule_format] :
+"
+  (((al, al'), (l :: ('a, 'b, 'c, 'd, 'e, 'f, 'g) ll list)) \<in> ll_validl_q \<longrightarrow>
+    (! n  ac ac' tc. n < length l \<longrightarrow> l ! n = ((ac, ac'), tc) \<longrightarrow>
+   (! cp nd nd' desc . 
+    ll_get_node ((ac, ac'), tc) cp = Some ((nd, nd'), desc) \<longrightarrow>
+    nd \<ge> al \<and> nd' \<le> al')))"
+  apply(insert qvalid_desc_bounded')
+  apply(fastforce)
+  done
+
+
 lemma valid3'_qvalid :
 "((x,t )  :: ('a, 'b, 'c, 'd, 'e) ll3') \<in> ll_valid3' \<Longrightarrow>
   ((x, t) :: ('a, 'b, 'c, 'd, 'e) ll3') \<in> ll_valid_q"
@@ -505,11 +530,695 @@ lemma valid3'_qvalid :
   apply(auto simp add:ll_valid_q_ll_validl_q.intros)
   done
 
+(* NB behavior of this function is perhaps counterintuitive
+for these purposes we consider a leaf node to be first child of itself *)
+(* i don't even know if we need this. *)
+fun firstchild :: "('a, 'b, 'c, 'd, 'e, 'f, 'g) ll \<Rightarrow> ('a, 'b, 'c, 'd, 'e, 'f, 'g) ll option"
+and firstchild_l :: "('a, 'b, 'c, 'd, 'e, 'f, 'g) ll list \<Rightarrow> ('a, 'b, 'c, 'd, 'e, 'f, 'g) ll option" where
+"firstchild (_, LSeq _ ls) = firstchild_l ls"
+| "firstchild T = Some T"
+| "firstchild_l [] = None"
+| "firstchild_l (h#t) =
+   (case firstchild h of
+         Some hc \<Rightarrow> Some hc
+         | None \<Rightarrow> firstchild_l t)"
+
+(* need auxiliary lemma, something like
+   if ((targstart, _), t) is descended from root
+   then when we pass the root through program_list_of_lst_validate
+   if t is not a Seq
+   then the instruction at index targstart (using the processed root)
+   is equal to t (where t is not a seq)
+    We could also define a 'first' function, and use that
+    to describe the Seq
+    (in fact if we define first appropriately we don't even need a case split
+      i think. just let first of any non seq thing be itself
+      first of a non-nil seq is first of its head
+      first of a nil sequence is ? ? (may make this more complicated))
+
+idea: what if first of a Nil sequence is None
+      and first of a sequence is the first of its first non-None argument
+      or None, if none are
+*)
+
+
+
+lemma qvalid_get_node' :
+"((((a, (t :: ('a, 'b, 'c, 'd, 'e, 'f, 'g) llt)) \<in> ll_valid_q) \<longrightarrow>
+    (! cp ad d . ll_get_node (a, t) cp = Some (ad, d) \<longrightarrow>
+    (ad, d) \<in> ll_valid_q)) \<and>
+ ((((a1, a2), (l:: ('a, 'b, 'c, 'd, 'e, 'f, 'g) ll list)) \<in> ll_validl_q \<longrightarrow> 
+    (! cp ad d . ll_get_node_list l cp = Some (ad, d) \<longrightarrow>
+    (ad, d) \<in> ll_valid_q))))"
+proof(induction rule:ll_valid_q_ll_validl_q.induct)
+case (1 i x e)
+  then show ?case 
+    apply(auto) apply(case_tac cp, auto simp add:ll_valid_q_ll_validl_q.intros)
+    done
+next
+  case (2 x d e)
+  then show ?case 
+    apply(auto) apply(case_tac cp, auto simp add:ll_valid_q_ll_validl_q.intros)
+done next
+  case (3 x d e s)
+  then show ?case
+    apply(auto) apply(case_tac cp, auto simp add:ll_valid_q_ll_validl_q.intros)
+    done
+next
+  case (4 x d e s)
+  then show ?case 
+    apply(auto) apply(case_tac cp, auto simp add:ll_valid_q_ll_validl_q.intros)
+    done
+next
+  case (5 n l n' e)
+  then show ?case 
+    apply(auto) apply(case_tac cp, auto simp add:ll_valid_q_ll_validl_q.intros)
+    done
+next
+  case (6 n)
+  then show ?case 
+    apply(auto) apply(case_tac cp, auto simp add:ll_valid_q_ll_validl_q.intros)
+    done
+next
+  case (7 n h n' t n'')
+  then show ?case 
+    apply(auto)
+    apply(case_tac cp, auto)
+    apply(case_tac aa, auto)
+    done
+qed
+
+lemma qvalid_get_node1 [rule_format] :
+"(((a, (t :: ('a, 'b, 'c, 'd, 'e, 'f, 'g) llt)) \<in> ll_valid_q) \<longrightarrow>
+    (! cp ad d . ll_get_node (a, t) cp = Some (ad, d) \<longrightarrow>
+    (ad, d) \<in> ll_valid_q))"
+  apply(insert qvalid_get_node'[of a t])
+  apply(auto)
+  done
+
+lemma inst_code_nonzero :
+"length (inst_code i) \<noteq> 0"
+  apply(case_tac i, auto)
+  apply(case_tac x10, auto)
+  apply(case_tac x2, auto)
+  apply(case_tac "31 < length list", auto)
+  done
+
+inductive ll_empty :: "('a, 'b, 'c, 'd, 'e, 'f, 'g) ll \<Rightarrow> bool" and
+          ll_emptyl :: "('a, 'b, 'c, 'd, 'e, 'f, 'g) ll list \<Rightarrow> bool" where
+"\<And> l x e . ll_emptyl l \<Longrightarrow> ll_empty (x, LSeq e l)"
+| "ll_emptyl []"
+| "\<And> h t . ll_empty h \<Longrightarrow> ll_emptyl t \<Longrightarrow> ll_emptyl (h#t)"
+
+lemma ll_qvalid_empty_r2l' :
+"(ll_empty (t :: ('a, 'b, 'c, 'd, 'e, 'f, 'g) ll) \<longrightarrow> 
+           (t \<in> ll_valid_q \<longrightarrow> (fst (fst t)) = (snd (fst t)))) \<and>
+ (ll_emptyl (l ::('a, 'b, 'c, 'd, 'e, 'f, 'g) ll list) \<longrightarrow> 
+           (! x x' . ((x, x'), l) \<in> ll_validl_q \<longrightarrow> x = x'))"
+proof(induction rule:ll_empty_ll_emptyl.induct)
+  case (1 l x e)
+  then show ?case
+    apply(auto)
+    apply(drule_tac ll_valid_q.cases) apply(auto)
+    done
+next
+ case 2
+  then show ?case
+    apply(auto) apply(drule_tac ll_validl_q.cases, auto)
+    done
+next
+  case (3 h t)
+  then show ?case
+    apply(auto)
+     apply(drule_tac ll_validl_q.cases, auto)
+ apply(drule_tac ll_validl_q.cases, auto)
+    done
+qed
+
+lemma ll_qvalid_empty_r2l2 [rule_format] :
+" (ll_emptyl (l ::('a, 'b, 'c, 'd, 'e, 'f, 'g) ll list) \<longrightarrow> 
+           (! x x' . ((x, x'), l) \<in> ll_validl_q \<longrightarrow> x = x'))"
+  apply(insert ll_qvalid_empty_r2l') apply(fastforce)
+  done
+
+lemma ll_qvalid_empty_l2r' :
+"(((x, t) :: ('a, 'b, 'c, 'd, 'e, 'f, 'g) ll) \<in> ll_valid_q \<longrightarrow> fst x = snd x \<longrightarrow>
+           (ll_empty (x, t))) \<and>
+ (((xl, xl'), (l ::('a, 'b, 'c, 'd, 'e, 'f, 'g) ll list)) \<in> ll_validl_q \<longrightarrow> xl = xl' \<longrightarrow>
+           (ll_emptyl l))"
+proof(induction rule:ll_valid_q_ll_validl_q.induct)
+case (1 i x e)
+  then show ?case apply(auto)
+    apply(case_tac i, auto)
+    apply(case_tac x10, auto)
+    apply(case_tac x2, auto)
+    apply(split if_split_asm) apply(auto)
+    done
+  next
+  case (2 x d e)
+  then show ?case 
+    apply(auto)
+    done
+next
+  case (3 x d e s)
+  then show ?case 
+    apply(auto)
+    done
+next
+  case (4 x d e s)
+  then show ?case 
+    apply(auto)
+    done
+next
+  case (5 n l n' e)
+  then show ?case 
+    apply(auto)
+    apply(auto simp add:ll_empty_ll_emptyl.intros)
+    done
+next
+  case (6 n)
+  then show ?case 
+    apply(auto simp add:ll_empty_ll_emptyl.intros)
+    done
+next
+  case (7 n h n' t n'')
+  then show ?case 
+    apply(auto)
+       apply(drule_tac qvalid_less1) apply(drule_tac qvalid_less2) apply(auto)
+      apply(drule_tac qvalid_less1) apply(drule_tac qvalid_less2) apply(auto)
+     apply(drule_tac qvalid_less1) apply(drule_tac qvalid_less2) apply(auto)
+    apply(drule_tac qvalid_less1) apply(drule_tac qvalid_less2) apply(auto)
+    apply(auto simp add:ll_empty_ll_emptyl.intros)
+    done
+qed
+
+(* we may need separate lemmas about the "load" function *)
+
+(* TODO: change last line to be about Forall rather than concat? *)
+lemma ll_empty_codegen_l2r' :
+"(ll_empty (t ::  ll4) \<longrightarrow> 
+           (! l' . codegen'_check t = Some l' \<longrightarrow> l' = [])) \<and>
+ (ll_emptyl (l :: ll4 list) \<longrightarrow> 
+    (! l' . List.those (List.map codegen'_check l) = Some l' \<longrightarrow> List.concat l' = []))
+"
+proof(induction rule:ll_empty_ll_emptyl.induct)
+case (1 l x e)
+  then show ?case apply(auto)
+    apply(split Option.option.split_asm, auto)
+    done
+next
+  case 2
+  then show ?case apply(auto)
+    done
+next
+  case (3 h t)
+  then show ?case apply(auto)
+    apply(case_tac "codegen'_check h", auto)
+    done
+qed
+
+lemma ll_empty_codegen_r2l' :
+"(codegen'_check (t ::  ll4) = Some [] \<longrightarrow> ll_empty t) \<and>
+ (! l' . List.those (List.map codegen'_check l) = Some l' \<longrightarrow> 
+    list_forall (\<lambda> x . x = []) l' \<longrightarrow> ll_emptyl l)
+"
+proof(induction rule:my_ll_induct)
+case (1 q e i)
+  then show ?case
+    apply(auto)
+    done
+next
+  case (2 q e idx)
+  then show ?case apply(auto) done
+next
+  case (3 q e idx n)
+  then show ?case apply(auto) done
+next
+  case (4 q e idx n)
+  then show ?case apply(auto) done
+next
+  case (5 q e l)
+  then show ?case apply(auto) 
+    apply(split option.split_asm) apply(auto)
+    apply(auto simp add:ll_empty_ll_emptyl.intros) done
+next
+  case 6
+then show ?case apply(auto simp add:ll_empty_ll_emptyl.intros) done
+next
+  case (7 h l)
+  then show ?case 
+    apply(auto)
+     apply(split option.split_asm, auto)
+    apply(split option.split_asm, auto)
+    apply(auto simp add:ll_empty_ll_emptyl.intros)
+    done
+qed
+
+lemma ll_empty_codegen_r2l1 [rule_format] :
+"(codegen'_check (t ::  ll4) = Some [] \<longrightarrow> ll_empty t)
+"
+  apply(insert ll_empty_codegen_r2l') apply(auto)
+  done
+
+
+lemma ll_empty_codegen_r2l2 [rule_format] :
+"(! l' . List.those (List.map codegen'_check l) = Some l' \<longrightarrow> 
+    list_forall (\<lambda> x . x = []) l' \<longrightarrow> ll_emptyl l)
+"
+  apply(insert ll_empty_codegen_r2l') apply(fastforce)
+  done
+
+
+lemma ll_nil_proglist_l2r :
+"program_list_of_lst_validate l = Some [] \<Longrightarrow> l = []"
+proof(induction l)
+  case Nil
+  then show ?case by auto
+next
+  case (Cons a l)
+  then show ?case apply(clarsimp)
+  apply(case_tac a, auto)
+             apply(split option.split_asm, auto)
+             apply(split option.split_asm, auto)
+             apply(split option.split_asm, auto)
+             apply(split option.split_asm, auto)
+            apply(split option.split_asm, auto)
+             apply(split option.split_asm, auto)
+             apply(split option.split_asm, auto)
+             apply(split option.split_asm, auto)
+        apply(split option.split_asm, auto)
+(* stack *) apply(case_tac x10, auto)
+         apply(split option.split_asm, auto)
+    apply(case_tac x2, auto) apply(split if_split_asm) apply(auto)
+        apply(split option.split_asm, auto)
+       apply(split option.split_asm, auto)
+      apply(split option.split_asm, auto)
+     apply(split option.split_asm, auto)
+    apply(split option.split_asm, auto)
+    done
+qed
+
+lemma ll_cons_proglist_l2r [rule_format] :
+"! h t . program_list_of_lst_validate l = Some (h#t) \<longrightarrow> (? t' . l = h#t')"
+proof(induction l)
+  case Nil
+  then show ?case by auto
+next
+  case (Cons a l)
+  then show ?case
+    apply(auto)
+    apply(case_tac a, auto)
+             apply(split option.split_asm, auto)
+             apply(split option.split_asm, auto)
+             apply(split option.split_asm, auto)
+             apply(split option.split_asm, auto)
+            apply(split option.split_asm, auto)
+             apply(split option.split_asm, auto)
+             apply(split option.split_asm, auto)
+             apply(split option.split_asm, auto)
+        apply(split option.split_asm, auto)
+(* stack *) apply(case_tac x10, auto)
+         apply(split option.split_asm, auto)
+    apply(case_tac x2, auto) apply(split if_split_asm) apply(auto)
+        apply(split option.split_asm, auto)
+       apply(split option.split_asm, auto)
+      apply(split option.split_asm, auto)
+     apply(split option.split_asm, auto)
+    apply(split option.split_asm, auto)
+    done
+qed
+
+(* TODO: finish this, this is a crucial next step *)
+(* used in the semantics to trick the PC into thinking everything is OK. *)
+(* this may have unintended side effects which will need to be debugged *)
+(* among other things, need to not allow codesize and extcodesize instructions,
+as these depend on already knowing the size of the code segment, which at the
+source level we do not *)
+definition bogus_prog :: program where
+"bogus_prog = Evm.program.make "(\<lambda> _ . 
+
+
+(* now we need a swapped version that takes ll_get_node as first premise *)
+(* see below for how we use rotate to do this *)
+
+(*
+if x2b is program_list_of_lst_validate (codegen' check x)
+and (q, d) is a descendent along childpath cp
+and let ch' = firstchild (q, d)
+then x2b ! (fst q) = ch'
+*)
+
+(* do we even need the firstchild thing? *)
+(* we aren't handling Seq [Seq []] correctly *)
+(* we are doing something wrong here, we should be able to handle
+the cases where the code buffer is empty more naturally, i suspect *)
+(*
+do we need to explicitly say adl < adr? that could possibly
+suffice at least for the non-Seq cases
+*)
+(*
+do we need to explicitly talk about program_list_of_lst?
+we shouldn't because the head should be the same in either case
+but it's possible relying on that makes things harder
+*)
+(*
+lemma program_list_of_lst_validate_correspond' :
+"((((a, (t :: ll4t)) \<in> ll_valid_q) \<longrightarrow>
+    (! cp adl adr d . ll_get_node (a, t) cp = Some ((adl, adr), d) \<longrightarrow>
+    (! il1 . codegen'_check (a,t) = Some il1 \<longrightarrow>
+    (! il2 . program_list_of_lst_validate il1 = Some il2 \<longrightarrow>
+          (? ilsub . codegen'_check ((adl, adr), d) = Some ilsub \<and>
+             (case ilsub of
+                   [] \<Rightarrow> adl = adr
+                   | ilh # ilt \<Rightarrow> 
+                      il2 ! (adl - fst a) = ilh \<and> adl \<ge> fst a)))))))
+\<and>
+
+(((((a1, a2), (l :: ll4 list)) \<in> ll_validl_q) \<longrightarrow>
+    (! cp adl adr d . ll_get_node_list l cp = Some ((adl, adr), d) \<longrightarrow>
+    (* not quite right - need to replace codegen'_check here *)
+    (! il1 e . codegen'_check ((a1, a2), LSeq e l) = Some il1 \<longrightarrow>
+    (! il2 . program_list_of_lst_validate il1 = Some il2 \<longrightarrow>
+          (? ilsub . codegen'_check ((adl, adr), d) = Some (ilsub) \<and>
+             (case ilsub of
+                   [] \<Rightarrow> adl = adr
+                  | ilh#ilt \<Rightarrow> il2 ! (adl - a1) = ilh \<and> adl \<ge> a1)))))))
+"*)
+
+(* is this lemma quite what we want? *)
+(* maybe we need a more specialized version specific to
+ll.L (instructions) *)
+lemma program_list_of_lst_validate_head' :
+"((((a, (t :: ll4t)) \<in> ll_valid_q) \<longrightarrow>
+    (! cp adl adr d . ll_get_node (a, t) cp = Some ((adl, adr), d) \<longrightarrow> adr > adl \<longrightarrow>
+    (! il1 . codegen'_check (a,t) = Some il1 \<longrightarrow>
+    (! il2 . program_list_of_lst_validate il1 = Some il2 \<longrightarrow>
+          (? ilh ilt . codegen'_check ((adl, adr), d) = Some (ilh#ilt) \<and>
+              il2 ! (adl - fst a) = ilh \<and> adl \<ge> fst a))))))
+\<and>
+
+(((((a1, a2), (l :: ll4 list)) \<in> ll_validl_q) \<longrightarrow>
+    (! cp adl adr d . ll_get_node_list l cp = Some ((adl, adr), d) \<longrightarrow> adr > adl \<longrightarrow>
+    (* not quite right - need to replace codegen'_check here *)
+    (! il1 e . codegen'_check ((a1, a2), LSeq e l) = Some il1 \<longrightarrow>
+    (! il2 . program_list_of_lst_validate il1 = Some il2 \<longrightarrow>
+          (? ilh ilt . codegen'_check ((adl, adr), d) = Some (ilh#ilt) \<and>
+             il2 ! (adl - a1) = ilh \<and> adl \<ge> a1))))))
+"
+proof(induction rule:ll_valid_q_ll_validl_q.induct)
+case (1 i x e)
+  then show ?case 
+    apply(auto)
+    apply(case_tac cp, auto)
+    apply(case_tac i, auto) apply(case_tac x10, auto)
+    apply(split if_split_asm, auto)
+     apply(split if_split_asm, auto)
+    apply(case_tac cp, auto)
+    done
+next
+  case (2 x d e)
+  then show ?case 
+    apply(auto)
+     apply(case_tac cp, auto)
+apply(case_tac cp, auto)
+    done
+next
+  case (3 x d e s)
+  then show ?case
+    apply(auto)
+     apply(case_tac cp, auto)
+apply(case_tac cp, auto)
+    done
+next
+  case (4 x d e s)
+  then show ?case
+    apply(auto)
+     apply(case_tac cp, auto)
+apply(case_tac cp, auto)
+    done
+next
+  case (5 n l n' e)
+  then show ?case
+    apply(clarify) apply(simp)
+    apply (split Option.option.split_asm, auto)
+    apply(case_tac cp, auto)
+    (* problem - now we don't know what the childpath is *)
+     apply(case_tac l, auto)
+      apply(drule_tac ll_validl_q.cases, auto)
+     apply(split Option.option.split_asm, auto)
+    (* seems kind of OK here... *)
+     apply(drule_tac program_list_of_lst_validate_split) apply(auto)
+     apply(frule_tac ll_validl_q.cases, auto)
+     apply(case_tac a', auto)
+      apply(case_tac b', auto)
+       apply(drule_tac ll_nil_proglist_l2r)
+apply(drule_tac ll_nil_proglist_l2r) apply(auto)
+       apply(drule_tac ll_empty_codegen_r2l1) apply(drule_tac ll_empty_codegen_r2l2) apply(auto)
+       apply(subgoal_tac "ll_emptyl (((n, n'a), h)#t)") apply(rule_tac [2] ll_empty_ll_emptyl.intros, auto)
+       apply(rotate_tac -1) apply(drule_tac ll_qvalid_empty_r2l2, auto)
+
+      apply(drule_tac ll_nil_proglist_l2r, auto)
+      apply(drule_tac ll_cons_proglist_l2r, auto)
+     apply(drule_tac ll_cons_proglist_l2r, auto)
+    apply(case_tac cp, auto)
+    done
+
+next
+  case (6 n)
+  then show ?case
+    apply(clarify)
+    apply(case_tac cp, auto)
+    done
+next
+  case (7 n h n' t n'')
+  then show ?case 
+    apply(clarify)
+    apply(case_tac cp, auto)
+
+     apply(split option.split_asm) apply(auto)
+
+      apply(split option.split_asm) apply(auto)
+      apply(split option.split_asm) apply(auto)
+     apply(split option.split_asm) apply(auto)
+     apply(split option.split_asm) apply(auto)
+     apply(case_tac a, auto)
+      apply(drule_tac x = list in spec) apply(auto)
+      apply(drule_tac program_list_of_lst_validate_split)
+      apply(auto)
+      apply(frule_tac qvalid_codegen'_check1) apply(auto)
+    (* to prove: adl \<le> n' (use "bounding" lemma?) *)
+    apply(frule_tac qvalid_desc_bounded1) apply(auto)
+      apply(subgoal_tac "adl - n < n' - n") apply(auto)
+      apply(subst nth_append) apply(auto)
+
+     apply(rotate_tac -4)
+     apply(drule_tac x = "nat # list" in spec) apply(auto)
+    apply(drule_tac program_list_of_lst_validate_split) apply(auto)
+           apply(frule_tac qvalid_codegen'_check1) apply(auto)
+     apply(subst nth_append) apply(auto)
+                
+    apply(split option.split_asm) apply(auto)
+     apply(split option.split_asm) apply(auto)
+     apply(split option.split_asm) apply(auto)
+    apply(split option.split_asm) apply(auto)
+    apply(split option.split_asm) apply(auto)
+    apply(case_tac a, auto)
+     apply(drule_tac qvalid_desc_bounded1, auto)
+    apply(frule_tac qvalid_less1, auto)
+    apply(rotate_tac -5)
+    apply(drule_tac x = "nat#list" in spec) apply(auto)
+    apply(drule_tac program_list_of_lst_validate_split) apply(auto)
+    done
+qed
+
+lemma program_list_of_lst_validate_head1 [rule_format] :
+"((((a, (t :: ll4t)) \<in> ll_valid_q) \<longrightarrow>
+    (! cp adl adr d . ll_get_node (a, t) cp = Some ((adl, adr), d) \<longrightarrow> adr > adl \<longrightarrow>
+    (! il1 . codegen'_check (a,t) = Some il1 \<longrightarrow>
+    (! il2 . program_list_of_lst_validate il1 = Some il2 \<longrightarrow>
+          (? ilh ilt . codegen'_check ((adl, adr), d) = Some (ilh#ilt) \<and>
+              il2 ! (adl - fst a) = ilh \<and> adl \<ge> fst a))))))"
+  apply(insert program_list_of_lst_validate_head')
+  apply(clarsimp)
+  done
+
+lemma ll_validl_snoc [rule_format]:
+"! x1 x2 tx1 tx2 t .
+   ((x1, x2), (l @ [((tx1, tx2), t)])) \<in> ll_validl_q \<longrightarrow>
+   (tx2 = x2 \<and>
+    ((x1, tx1), l) \<in> ll_validl_q \<and>
+    ((tx1, x2), t) \<in> ll_valid_q)
+"
+proof(induction l)
+case Nil
+  then show ?case
+    apply(auto)
+      apply(drule_tac ll_validl_q.cases, auto)
+      apply(drule_tac ll_validl_q.cases, auto)
+     apply(drule_tac ll_validl_q.cases, auto)
+    apply(rule_tac ll_valid_q_ll_validl_q.intros)
+    apply(drule_tac ll_validl_q.cases, auto)
+    apply(drule_tac ll_validl_q.cases, auto)
+    done
+next
+  case (Cons a l)
+  then show ?case 
+    apply(auto)
+      apply(drule_tac ll_validl_q.cases, auto)
+     apply(drule_tac ll_validl_q.cases, auto)
+     apply(drule_tac x = n' in spec)
+     apply(drule_tac x = n'' in spec)
+     apply(drule_tac x = tx1 in spec)
+     apply(drule_tac x = tx2 in spec) 
+apply(drule_tac x = t in spec)
+     apply(auto simp add:ll_valid_q_ll_validl_q.intros)
+
+    apply(drule_tac ll_validl_q.cases, auto)
+  
+  done
+qed
+
+lemma ll_valid_app [rule_format] :
+"! x1 x2 l1 . ((x1, x2), (l1 @ l2)) \<in> ll_validl_q \<longrightarrow>
+  (? mid . ((x1, mid), l1) \<in> ll_validl_q \<and>
+           ((mid, x2), l2) \<in> ll_validl_q)
+"
+proof(induction l2)
+  case Nil
+  then show ?case
+    apply(auto) apply(rule_tac x = x2 in exI, auto)
+    apply(rule_tac ll_valid_q_ll_validl_q.intros)
+    done
+next
+  case (Cons a l2)
+  then show ?case 
+    apply(auto) apply(case_tac a, auto)
+    apply(drule_tac x = x1 in spec) apply(drule_tac x = x2 in spec)
+    apply(drule_tac x = "l1 @ [((aa, b), ba)]" in spec) apply(auto)
+    apply(rule_tac x = aa in exI) apply(auto)
+     apply(frule_tac ll_validl_snoc, auto)
+    apply(frule_tac ll_validl_snoc, auto)
+    apply(auto simp add:ll_valid_q_ll_validl_q.intros)
+    done
+qed
+
+(*
+some additional lemmas about non-empty things (using emptiness directly
+seems annoying sometimes)
+*)
+lemma ll_L_valid_bytes_length:
+"((x, L e i) \<in> ll_valid_q \<Longrightarrow> fst x < snd x)
+"  
+  apply(drule_tac ll_valid_q.cases)
+       apply(auto)
+  apply(subgoal_tac "length (inst_code i) \<noteq> 0") apply(rule_tac[2] inst_code_nonzero)
+  apply(auto)
+  done
+
+
+(*
+lemma about case where cp_next is None
+this means that (if we are a descendent of a qvalid root)
+our ending annotation is equal to the overall ending annotation
+
+(we may need a similar lemma characterizing the case where cp_next is Some)
+(that is, that our ending annotation is equal to the start annotation of
+our cp_next)
+*)
+
+(*
+it's possible this is not necessary?
+*)
+
+(*
+lemma qvalid_cp_next_None' :
+"(((x, t) :: ('a, 'b, 'c, 'd, 'e, 'f, 'g) ll) \<in> ll_valid_q \<longrightarrow>
+  (! cp xd d . ll_get_node (x, t) cp = Some (xd, d) \<longrightarrow>
+    cp_next (x, t) cp = None \<longrightarrow>
+    snd x = snd xd)) 
+\<and>
+(((x1, x2), (l :: ('a, 'b, 'c, 'd, 'e, 'f, 'g) ll list)) \<in> ll_validl_q \<longrightarrow>
+  (! cp xd d . ll_get_node_list l cp = Some (xd, d) \<longrightarrow>
+    (! e . cp_next ((x1, x2), LSeq e l) cp = None \<longrightarrow>
+    snd x = snd xd)))"
+proof(induction rule:ll_valid_q_ll_validl_q.induct)
+case (1 i x e)
+  then show ?case 
+    apply(auto)
+    apply(case_tac "rev cp", auto)
+    apply(case_tac "rev list", auto)
+    done
+next
+  case (2 x d e)
+  then show ?case 
+      apply(auto)
+    apply(case_tac "rev cp", auto)
+    apply(case_tac "rev list", auto)
+    done
+next
+  case (3 x d e s)
+  then show ?case 
+    apply(auto)
+    apply(case_tac "rev cp", auto)
+    apply(case_tac "rev list", auto)
+    done
+next
+  case (4 x d e s)
+  then show ?case
+    apply(auto)
+    apply(case_tac "rev cp", auto)
+    apply(case_tac "rev list", auto)
+    done
+next
+  case (5 n l n' e)
+  then show ?case 
+    apply(auto)
+    apply(case_tac "rev cp", auto)
+    apply(case_tac "rev list", auto)
+     apply(drule_tac x = "[aa]" in spec) apply(auto)
+     apply(case_tac "ll_get_node_list l [Suc aa]") apply(auto)
+    (* idea: aa'th tail of l must also be valid *)
+    (* maybe we can use different conditions on the child path to make proving easier *)
+    (* one proof approach: 2 lemmas:
+        1. if our child path has no successor, we must be the last thing in the list (maybe not even needed, could be trivial)
+        2. a "splitting" lemma for validl_q along append (@)
+maaaaybe we can just use descend bound?
+    *)
+(* the lemmas from above didn't quite work.
+the issue is relating get_node to a position in the listn. *)
+     apply(case_tac aa, auto) apply(case_tac l, auto) apply(case_tac list, auto)
+    apply(drule_tac ll_validl_q.cases, auto) apply(drule_tac ll_validl_q.cases, auto)
+next
+  case (6 n)
+  then show ?case sorry
+next
+  case (7 n h n' t n'')
+  then show ?case sorry
+qed
+*)
+(*
+lemma qvalid_cp_next_Some' :
+
+lemma qvalid_cp_next_Some1 :
+*)
+
 (*
 idea: don't use program_map_of_lst?
 maybe just use program_list_of_lst with index?
 it would be nice to be able to use the "bang" notation,
 but maybe LemExtraDefs.index is the way to go?
+*)
+(*
+don't use ll_load_lst_validate
+instead create one that defines its program as being
+equal to the compiled program
+but that seems sketchy, relying on compiled
+code to specify source language semantics
+*)
+(*
+another option: use a bogus program for our input such that vctx_advance_pc
+will always advance the pc by 1 (of course this will mean nothing)
+idea: program is just an infinite stream of noops (?)
 *)
 lemma elle_alt_correct :
 "elle_alt_sem ((t :: ll4)) intp cp est est' (* (ir, cc, net) (ir', cc', net') *) \<Longrightarrow>
@@ -519,8 +1228,10 @@ lemma elle_alt_correct :
  intp = elle_interp \<longrightarrow>
  (! targstart targend tdesc . ll_get_node t cp = Some ((targstart, targend), tdesc) \<longrightarrow>
    (! vi . fst est = InstructionContinue vi \<longrightarrow>
+    (* require that prog already be loaded beofre this point? *)
+   (! prog . ll4_load_lst_validate (fst (snd est)) t = Some prog \<longrightarrow>
    (! act vc venv fuel stopper . program_sem stopper
-               (ll4_load_lst_cctx (fst (snd est)) t) 
+               prog 
                fuel (snd (snd est)) 
 (* is this arithmetic around fst (fst t) right? *)
 (* perhaps we need a secondary proof that validity implies
@@ -529,20 +1240,206 @@ that targstart will be greater than or equal to fst (fst t) *)
                    (* fuel can be arbitrary, but we require to compute to a final result *)
                    InstructionToEnvironment act vc venv \<longrightarrow>
                   (* the issue may have to do with distinguishing between errors? *)
-                  setpc_ir (fst est') 0 = setpc_ir (InstructionToEnvironment act vc venv) 0)))))"
+                  (* TODO: in some cases we end up having to compare unloaded programs? *)
+                  setpc_ir (fst est') 0 = setpc_ir (InstructionToEnvironment act vc venv) 0))))))"
 proof(induction rule:elle_alt_sem.induct)
 case (1 t cp x e i instD jmpD jmpiD labD st st')
   then show ?case 
     apply(clarify)
     apply(subgoal_tac "(x, llt.L e i) = ((targstart, targend), tdesc)") apply(auto)
 
+
     apply(case_tac fuel, auto)
      apply(split Option.option.split_asm) apply(auto)
       apply(split Option.option.split_asm) apply(auto)
      apply(split Option.option.split_asm) apply(auto)
-     apply(simp split:if_split_asm) apply(auto)
-         apply(simp_all add:program.defs)
+     apply(split Option.option.split_asm) apply(auto)
+     apply(split Option.option.split_asm) apply(auto)
+     apply(split Option.option.split_asm) apply(auto)
 
+     apply(split if_split_asm, auto)
+         apply(simp add:program.defs)
+         apply(frule_tac valid3'_qvalid)
+         apply(frule_tac qvalid_desc_bounded1, auto)
+    apply(frule_tac qvalid_codegen'_check1, auto)
+    (* idea for a contradiction here: descended guy must be qvalid
+       but, we also know targstart = targend \<rightarrow> contradicts the fact
+       that this must be an instruction *)
+         apply(drule_tac qvalid_get_node1[rotated 1], auto)
+    apply(rotate_tac -1)
+         apply(drule_tac ll_valid_q.cases) apply(auto)
+         apply(subgoal_tac "length (inst_code i) \<noteq> 0")
+          apply(rule_tac[2] inst_code_nonzero) apply(auto)
+
+(* next up: contradictory cases where program_content doesn't have
+the instruction at targstart (last few thms should be useful) *)
+        apply(simp add:program.defs)
+         apply(frule_tac valid3'_qvalid)
+         apply(frule_tac qvalid_desc_bounded1, auto)
+        apply(frule_tac qvalid_codegen'_check1, auto)
+         apply(drule_tac qvalid_get_node1[rotated 1], auto)
+    apply(rotate_tac -1)
+         apply(drule_tac ll_valid_q.cases) apply(auto)
+         apply(subgoal_tac "length (inst_code i) \<noteq> 0")
+         apply(rule_tac[2] inst_code_nonzero) apply(auto)
+
+        apply(simp add:program.defs)
+         apply(frule_tac valid3'_qvalid)
+         apply(frule_tac qvalid_desc_bounded1, auto)
+        apply(frule_tac qvalid_codegen'_check1, auto)
+         apply(drule_tac qvalid_get_node1[rotated 1], auto)
+    apply(rotate_tac -1)
+         apply(drule_tac ll_valid_q.cases) apply(auto)
+         apply(subgoal_tac "length (inst_code i) \<noteq> 0")
+        apply(rule_tac[2] inst_code_nonzero) apply(auto)
+
+        apply(simp add:program.defs)
+         apply(frule_tac valid3'_qvalid)
+         apply(frule_tac qvalid_desc_bounded1, auto)
+        apply(frule_tac qvalid_codegen'_check1, auto)
+         apply(drule_tac qvalid_get_node1[rotated 1], auto)
+    apply(rotate_tac -1)
+         apply(drule_tac ll_valid_q.cases) apply(auto)
+         apply(subgoal_tac "length (inst_code i) \<noteq> 0")
+       apply(rule_tac[2] inst_code_nonzero) apply(auto)
+
+        apply(simp add:program.defs)
+         apply(frule_tac valid3'_qvalid)
+         apply(frule_tac qvalid_desc_bounded1, auto)
+        apply(frule_tac qvalid_codegen'_check1, auto)
+         apply(drule_tac qvalid_get_node1[rotated 1], auto)
+    apply(rotate_tac -1)
+         apply(drule_tac ll_valid_q.cases) apply(auto)
+         apply(subgoal_tac "length (inst_code i) \<noteq> 0")
+      apply(rule_tac[2] inst_code_nonzero) apply(auto)
+
+(* final goal *)
+    apply( split if_split_asm)
+    apply(clarsimp)
+(* seems OK up to here. *)
+     apply(simp add:program.defs) apply(clarsimp)
+     apply(frule_tac valid3'_qvalid)
+     apply(frule_tac qvalid_get_node1) apply(simp)
+     apply(rotate_tac -1)
+     apply(frule_tac ll_L_valid_bytes_length) apply(simp)
+     
+    (* idea - here we need to do the following:
+       1. use qvalid desc to get the fact that our descendent is qvalid
+       2. use this + fact desc is an L to get that it targstart < targend 
+          - "emptiness" lemmas may help
+       3. now we can apply program_list_of_lst_validate_head1
+       now, do a case split on i to figure out what the instruction actually is.
+*)
+    apply(rotate_tac 1)
+     apply(frule_tac t = ttree and cp = cp and d = " llt.L () i" in program_list_of_lst_validate_head1)
+         apply(simp)
+        apply(simp) apply(simp) apply(simp)
+    apply(simp)
+     apply(simp_all)
+     apply(clarify)
+     apply(simp add: elle_interp_def) apply(clarify)
+
+(* i think this is OK up to here. *)
+     apply(case_tac st)
+(* cases for each instruction *)
+     apply(case_tac "x2b ! targstart")
+                 apply(simp add:check_resources_def)
+                 apply(clarsimp)
+                apply(clarsimp)
+(* something weird is going on here - we are ending up having
+to compare the resultant state to one that doesn't have the
+program loaded... this leads me to think our theorem statement is wrong *)
+                   apply(simp add:check_resources_def)
+                apply(case_tac x2a) apply(clarsimp)
+                    apply(case_tac "vctx_stack vi") apply(clarsimp)
+                    apply(clarsimp) apply(case_tac list) apply(clarsimp) (* False goal emerges here *) apply(clarsimp) 
+                    apply(simp add:program.defs) apply(split option.split_asm)
+    apply(split option.split_asm)         
+                      apply(clarsimp) apply(clarsimp) apply(simp add:program.defs)
+    apply(split option.split_asm)
+                     apply(clarsimp)
+    apply(simp)
+(* to draw a contradiction here, i need to show the instruction must be the last one *)
+    apply(simp)
+(*
+                 apply(case_tac n) apply(simp)
+                  apply(case_tac st) apply(simp) apply(split if_split_asm)
+    apply(simp) apply(fastforce)
+
+                  apply(simp)
+                  apply(split if_split_asm)
+                   apply(split if_split_asm) apply(simp)
+                    apply(simp add:check_resources_def)
+                   apply(simp add:check_resources_def)
+                  apply(split if_split_asm)
+                   apply(simp add:check_resources_def)
+    apply(case_tac "vctx_gas vi") apply(auto)
+(* uh oh. is there a problem with our error cases?
+e.g. returning the wrong list of error reasons?
+*)
+    apply(fastforce)    
+   (* apply(case_tac i)*)
+  (* what follows here is quite repetitive, perhaps there is a nice way to do all these steps
+compactly. *)
+(*
+                        apply(clarsimp)
+                        apply(simp add:elle_interp_def)
+                        apply(case_tac x1, auto)
+                        apply(case_tac n, auto)
+                        apply(case_tac st, auto)
+                        apply(simp add:check_resources_def)
+apply(case_tac st, auto)
+                        apply(simp add:check_resources_def)
+    apply(simp add:elle_interp_def)
+                       apply(case_tac x2a, auto)
+    apply(case_tac "vctx_stack vi", auto)
+                        apply(case_tac st, auto)   
+                        apply(simp add:check_resources_def)
+                        apply(case_tac list, auto)
+                        apply(simp add:check_resources_def)
+                        apply(case_tac st, auto)
+                        apply(simp add:check_resources_def)
+    apply(case_tac st, auto)
+                        apply(simp add:check_resources_def)
+                        apply(split list.split_asm) apply(auto)
+apply(split list.split_asm) apply(auto)
+*)
+
+(* now we need to show we are at the end.
+this should be doable using some facts about
+cp_next *)
+(* could be as simple as a lemma that says
+"if we are valid and cp_next = None, then
+we must be the last item *)
+    apply(hypsubst cp_next.simps)
+    apply(case_tac x1, clarsimp)
+
+(* proof needs to talk about x2b ! targstart 
+specifically, if x2b is program_list_of_lst_validate (codegen' check x)
+and (q, d) is a descendent along childpath cp
+and let ch' = firstchild (q, d)
+then x2b ! (fst q) = ch'
+*)
+
+(* also need to prove x2b is non nil
+proof sketch:
+1. ttree has a descended llt.L
+2. this descended llt.L must be qvalid \<rightarrow> targend > targstart
+3. because of descended boundnedness lemma, 0 \<le> targstart < targend \<le> tend
+4. with an extra lemma (?) this will show us that x2b ! targstart exists (?)
+*)
+
+(* let's make sure we have everything we need here before we prove
+that theorem.
+*)
+     apply(simp add:program.defs) apply(clarsimp)
+
+      (* need to prove i = x2a or something like that *)
+     apply(case_tac x2a)
+    apply(simp)
+     apply(auto)
+    apply(auto)
+    apply(clarify)
 
 (*
 another phrasing of the lemmas we need
